## First-Order Linear Diff. Equation

The form:
$$
{dy\over dt} + p(t)y = g(t)
$$

Take the `integral factor` $\mu(t)$, then we have:
$$
\mu(t){dy\over dt} + \mu(t)p(t)y = \mu(t)g(t)
$$
We know the `fact` that
$$
{d (\mu(t)y) \over dt} = \mu(t){dy\over dt} + {d\mu(t)\over dt}y
$$
Put this two equation above together, we have obtained
$$
{d (\mu(t)y) \over dt} - {d\mu(t)\over dt}y + \mu(t)p(t)y = \mu(t)g(t)
$$

In order to make the 2nd and 3rd term be equal, we have the `condition`:
$$
{d\mu(t)\over dt}y = \mu(t)p(t)y
$$
such that the left side of the equation becomes
$$
{d (\mu(t)y) \over dt} + 0 = \mu(t)g(t)
$$

Then, calculate the `condition` for $\mu(t)$:

$$
\begin{aligned}
{d\mu(t)\over dt} &= \mu(t)p(t) \\
{d\mu(t)\over \mu(t)} &= p(t)dt \\
d\ln |\mu(t)| &= p(t)dt \\
\int d\ln |\mu(t)| &= \int p(t)dt \\
\ln |\mu(t)| &= \int p(t)dt + C \\
\mu(t) &= \exp[\int p(t)dt + C]
\end{aligned}
$$

Then
$$
\begin{aligned}
{d (\mu(t)y) \over dt} + 0 &= \mu(t)g(t) \\
\mu(t)y &= \int \mu(t)g(t)dt + C\\
y &= {1\over \mu(t)} \left[\int_{t_0}^t \mu(s)g(s)ds + C\right]
\end{aligned}
$$
Put the conditon $\mu(t)$ into this formula, then we can solve this equation for $y$.


### 常数变易法 Variation of parameters \ method of constant variations.
